checkpoint generalized plan that may support layering/abstractions/rep functions

src/BasicSecurity.v
@@ -311,3 +311,266 @@ Proof.
   inversion H4; subst.
   eauto.
 Qed.
+
+Require Import Array.
+
+Definition rep partA partB :=
+  (arrayN ptsto_subset 0 partA *
+   arrayN ptsto_subset (length partA) partB)%pred.
+
+Definition read_partA a :=
+  Read a.
+
+Definition write_partA a v :=
+  Write a v.
+
+
+Definition prog_secureF T PreSameT PostSameT CrashSameT FT
+  (p : prog T)
+  (pre : PreSameT -> FT -> rawpred)
+  (post : PostSameT -> FT -> rawpred)
+  (crash : CrashSameT -> FT -> rawpred) :=
+
+  forall m1 m2 presame F1 F2 out1 vm hm,
+
+  pre presame F1 m1 ->
+  pre presame F2 m2 ->
+  exec m1 vm hm p out1 ->
+
+  (exists r m1' m2' vm' hm' postsame,
+   out1 = Finished m1' vm' hm' r /\
+   exec m2 vm hm p (Finished m2' vm' hm' r) /\
+   post postsame F1 m1' /\
+   post postsame F2 m2') \/
+
+  (exists m1' m2' hm' crashsame,
+   out1 = Crashed _ m1' hm' /\
+   exec m2 vm hm p (Crashed _ m2' hm') /\
+   crash crashsame F1 m1' /\
+   crash crashsame F2 m2').
+
+Theorem read_secureF:
+  forall (a:addr),
+  prog_secureF (Read a)
+               (fun mp F => F * diskIs mp * [[ a |+>? mp ]])%pred
+               (fun mp F => F * diskIs mp * [[ a |+>? mp ]])%pred
+               (fun mp F => F * diskIs mp * [[ a |+>? mp ]])%pred.
+Proof.
+  unfold prog_secureF; intros.
+  destruct_lift H.
+  destruct_lift H0.
+  inv_exec.
+  - (* Finished *)
+    left.
+    unfold ptsto_subset in H2; destruct_lift H2.
+    repeat eexists.
+    + econstructor.
+      econstructor.
+      rewrite (diskIs_pred _ H1) in H0.
+      rewrite (diskIs_pred _ H1) in H.
+      eapply ptsto_valid' in H.
+      eapply ptsto_valid' in H0.
+      rewrite H9 in H; inversion H; subst.
+      eauto.
+    + eapply sep_star_lift_apply'; eauto.
+      unfold ptsto_subset; pred_apply; cancel.
+    + eapply sep_star_lift_apply'; eauto.
+      unfold ptsto_subset; pred_apply; cancel.
+  - (* Failed *)
+    exfalso.
+    rewrite (diskIs_pred _ H2) in H.
+    destruct_lift H.
+    eapply ptsto_subset_valid' in H.
+    repeat deex.
+    congruence.
+  - (* Crashed *)
+    right.
+    repeat eexists; eauto.
+    eapply sep_star_lift_apply'; eauto; pred_apply; cancel.
+    eapply sep_star_lift_apply'; eauto; pred_apply; cancel.
+Qed.
+
+Theorem write_secureF:
+  forall (a:addr) v,
+  prog_secureF (Write a v)
+               (fun mp F => F * diskIs mp * [[ a |+>? mp ]])%pred
+               (fun mp F => F * diskIs mp * [[ (exists v0, a |+> (v, vsmerge v0))%pred mp ]])%pred
+               (fun mp F => F * diskIs mp * [[ a |+>? mp ]])%pred.
+Proof.
+  unfold prog_secureF; intros.
+  destruct_lift H.
+  destruct_lift H0.
+  inv_exec.
+  - (* Finished *)
+    left.
+    unfold ptsto_subset in H2; destruct_lift H2.
+    repeat eexists.
+    + econstructor.
+      econstructor.
+      rewrite (diskIs_pred _ H1) in H0.
+      rewrite (diskIs_pred _ H1) in H.
+      eapply ptsto_valid' in H.
+      eapply ptsto_valid' in H0.
+      rewrite H14 in H; inversion H; subst.
+      eauto.
+    + eapply sep_star_lift_apply'; eauto.
+      eapply diskIs_sep_star_upd. 2: eauto.
+      unfold ptsto in H1; intuition eauto.
+      exists (v2, x).
+      apply emp_star.
+      eapply ptsto_subset_upd.
+      clear H1. pred_apply; cancel.
+      apply incl_refl.
+    + rewrite diskIs_pred in H; eauto.
+      eapply ptsto_valid' in H.
+      rewrite H14 in H; inversion H; subst.
+      eapply sep_star_lift_apply'; eauto.
+      eapply diskIs_sep_star_upd. 2: eauto.
+      unfold ptsto in H1; intuition eauto.
+      exists (dummy_cur, dummy).
+      apply emp_star.
+      eapply ptsto_subset_upd.
+      clear H1. pred_apply; cancel.
+      apply incl_refl.
+  - (* Failed *)
+    exfalso.
+    rewrite (diskIs_pred _ H2) in H.
+    destruct_lift H.
+    eapply ptsto_subset_valid' in H.
+    repeat deex.
+    congruence.
+  - (* Crashed *)
+    right.
+    repeat eexists; eauto.
+    eapply sep_star_lift_apply'; eauto; pred_apply; cancel.
+    eapply sep_star_lift_apply'; eauto; pred_apply; cancel.
+Qed.
+
+Theorem ret_secureF:
+  forall T (x : T),
+  prog_secureF (Ret x)
+               (fun (mp : unit) F => F)
+               (fun (mp : unit) F => F)
+               (fun (mp : unit) F => F).
+Proof.
+  unfold prog_secureF; intros.
+  inv_exec.
+  left.
+  do 6 eexists; intuition.
+Qed.
+
+Theorem bind_secureF:
+  forall T1 T2 TP1 TP2 TP3 TP4 TF (p1 : prog T1) (p2 : T1 -> prog T2) (pre : TP1 -> TF -> _)
+      (post1 : TP2 -> TF -> _)
+      (post2 : TP3 -> TF -> _)
+      (crash : TP4 -> TF -> _),
+  prog_secureF p1 pre post1 crash ->
+  (forall x, prog_secureF (p2 x) post1 post2 crash) ->
+  prog_secureF (Bind p1 p2) pre post2 crash.
+Proof.
+  unfold prog_secureF; intros.
+  inv_exec.
+  - (* p1 Finished *)
+    specialize (H _ _ _ _ _ _ _ _ H1 H2 H10).
+    intuition; repeat deex; try congruence.
+    inversion H3; subst.
+    specialize (H0 r _ _ _ _ _ _ _ _ H4 H6 H13).
+    intuition; repeat deex.
+    + left.
+      do 6 eexists; intuition eauto.
+    + right.
+      do 4 eexists; intuition eauto.
+  - (* p1 Failed *)
+    specialize (H _ _ _ _ _ _ _ _ H1 H2 H9).
+    intuition; repeat deex; try congruence.
+  - (* p1 Crashed *)
+    specialize (H _ _ _ _ _ _ _ _ H1 H2 H9).
+    intuition; repeat deex; try congruence.
+    right.
+    inversion H3; subst.
+    do 4 eexists; intuition.
+    constructor.
+    eauto.
+    eauto.
+    eauto.
+Qed.
+
+(*
+Theorem frame_secureF:
+  forall T (p : prog T) pre post F,
+  prog_secureF p pre post ->
+  prog_secureF p (F * pre)%pred (F * post)%pred.
+Proof.
+  unfold prog_secure; intros.
+  eapply diskIs_sep_star_split in H2; repeat deex; intuition.
+  rewrite H6 in H0.
+  rewrite H6 in H1.
+  apply sep_star_assoc in H0.
+  apply sep_star_assoc in H1.
+  specialize (H _ _ _ _ _ _ _ _ H0 H1 H2 H3).
+  intuition; repeat deex.
+  - left.
+    apply sep_star_assoc in H7.
+    apply sep_star_assoc in H8.
+    rewrite (diskIs_sep_star_combine _ _ H4 H10) in H7; destruct_lift H7.
+    rewrite (diskIs_sep_star_combine _ _ H4 H10) in H8; destruct_lift H8.
+    do 6 eexists; intuition eauto.
+  - right.
+    apply sep_star_assoc in H7.
+    apply sep_star_assoc in H9.
+    assert ((diskIs mc) mc) by congruence.
+    rewrite (diskIs_sep_star_combine _ _ H4 H5) in H7; destruct_lift H7.
+    rewrite (diskIs_sep_star_combine _ _ H4 H5) in H9; destruct_lift H9.
+    do 4 eexists; intuition eauto.
+Qed.
+*)
+
+Theorem pimpl_secureF:
+  forall T (p : prog T) TPre TPost TCrash TF TF'
+           (pre : TPre -> TF -> _) (pre' : TPre -> TF' -> _)
+           (post : TPost -> TF -> _) (post' : TPost -> TF' -> _)
+           (crash : TCrash -> TF -> _) (crash' : TCrash -> TF' -> _)
+           (XF : TF' -> TF),
+  (forall presame F, pre' presame F =p=> pre presame (XF F)) ->
+  (forall postsame F, post postsame (XF F) =p=> post' postsame F) ->
+  (forall crashsame F, crash crashsame (XF F) =p=> crash' crashsame F) ->
+  prog_secureF p pre post crash ->
+  prog_secureF p pre' post' crash'.
+Proof.
+  unfold prog_secureF; intros.
+  apply H in H3.
+  apply H in H4.
+  specialize (H2 _ _ _ _ _ _ _ _ H3 H4 H5).
+  intuition; repeat deex.
+  - left.
+    do 6 eexists; intuition eauto.
+    eapply H0. eauto.
+    eapply H0. eauto.
+  - right.
+    do 4 eexists; intuition eauto.
+    eapply H1; eauto.
+    eapply H1; eauto.
+Qed.
+
+
+Require Import GenSepN.
+
+Theorem read_partA_secure :
+  forall (a:addr),
+  prog_secureF (read_partA a)
+               (fun mp '(Ftop, Fp, partB) => (exists partA, Ftop * rep partA partB * [[ (Fp * diskIs mp)%pred (list2nmem partA) ]] * [[ (a |+>?)%pred mp ]])%pred)
+               (fun mp '(Ftop, Fp, partB) => (exists partA, Ftop * rep partA partB * [[ (Fp * diskIs mp)%pred (list2nmem partA) ]] * [[ (a |+>?)%pred mp ]])%pred)
+               (fun mp '(Ftop, Fp, partB) => (exists partA, Ftop * rep partA partB * [[ (Fp * diskIs mp)%pred (list2nmem partA) ]] * [[ (a |+>?)%pred mp ]])%pred).
+Proof.
+  intros.
+  unfold rep.
+  eapply pimpl_secureF.
+  4: eapply read_secureF.
+
+  destruct F; destruct p; intros.
+  cancel.
+  rewrite (diskIs_pred _ H1) in H2.
+  rewrite arrayN_except.
+  2: unfold ptsto_subset in H2; destruct_lift H2; eapply list2nmem_inbound in H; eauto.
+  
+  Search arrayN arrayN_ex.
